Progress.v
@@ -47,66 +47,330 @@ Proof.
   simpl. destruct cns; reflexivity.
   Qed.
 
+Theorem mkChangesHaltsOnHalt : forall chs, mkChanges halt chs = Some halt.
+Proof.
+  induction chs. reflexivity. simpl. assumption. Qed.
+
+Theorem mkChangesStuckOnStuck : forall chs, mkChanges stuck chs = Some stuck.
+Proof.
+  induction chs. reflexivity. simpl. assumption. Qed.
+
+Inductive isUpdateFrameVal : deltaState -> Prop :=
+  upValProp : forall n v, isUpdateFrameVal (updateFrame (upVals n v)).
+
+Theorem mkChangesProgressOnUpdateFrameValPairs : forall l, forAllList l isUpdateFrameVal ->
+  forall rvs m pc frms h sh inb outb,
+  exists rvs',
+  mkChanges (dst (frm rvs m pc :: frms) h sh inb outb) l = Some (dst (frm rvs' m pc :: frms) h sh inb outb).
+Proof.
+  intros l H.
+  induction l.
+    eexists; simpl; reflexivity.
+    simpl. inversion H. destruct a; try inversion H2.
+    intros. destruct (VLIST.find (n, v) compFirst rvs);
+    eapply IHl; assumption.
+  Qed. 
+
+Theorem evalHpInstHeapEq : forall loc1 h,EVAL.HP.get loc1 h = INSTRUCTION.HEAP.get loc1 h.
+Proof.
+  intros.
+  unfold EVAL.HP.get. unfold INSTRUCTION.HEAP.get. reflexivity.
+Qed.
+
+Theorem progressNop : forall (st:DVMState) (p:Program), consistentNop st p -> 
+  (exists st',INSTRUCTION.stepWith nop st p = Some st' /\ ~(st' = stuck)).
+Proof.
+  destruct st.
+  intros. inversion H. unfold INSTRUCTION.stepWith. unfold INSTRUCTION.evalInst.
+  unfold INSTRUCTION.evalNop. rewrite H6. rewrite H7. simpl. eexists. split. reflexivity.
+  intro Contra; inversion Contra.
+  intros. inversion H. intros. eexists. split. reflexivity. intro Contra; inversion Contra.
+Qed.
+
+Theorem progressRet : forall (st:DVMState) (p:Program), consistentRet st p -> 
+  (exists st',INSTRUCTION.stepWith ret st p = Some st' /\ ~(st' = stuck)).
+Proof.
+  destruct st; intros. inversion H. unfold INSTRUCTION.stepWith. unfold INSTRUCTION.evalInst.
+  unfold INSTRUCTION.evalRet. rewrite H6. rewrite H7.
+  destruct (EVAL.evalReg 201 (dst (f :: frm vals ml pc :: frms0) h sh inb outb)).
+    remember (upVals 201 v) as trv.
+    simpl. destruct trv.
+    destruct (VLIST.find (n, v0) compFirst vals). simpl. eexists.
+    split. reflexivity. intro Contra. inversion Contra.
+    eexists. split. reflexivity. intro Contra. inversion Contra.
+    inversion Heqtrv.
+    eexists. split. reflexivity. intro Contra. inversion Contra.
+    inversion H. eexists. split. reflexivity. intro Contra. inversion Contra.
+Qed.  
+
+Theorem progressRetTo : forall (st:DVMState) (p:Program) r, consistentRet st p -> 
+  (exists st',INSTRUCTION.stepWith (retTo r) st p = Some st' /\ ~(st' = stuck)).
+Proof.
+  destruct st; intros. inversion H. unfold INSTRUCTION.stepWith. unfold INSTRUCTION.evalInst.
+  unfold INSTRUCTION.evalRetTo. rewrite H6. rewrite H7.
+  destruct (EVAL.evalReg 201 (dst (f :: frm vals ml pc :: frms0) h sh inb outb)).
+    remember (upVals r v) as trv.
+    simpl. destruct trv.
+    destruct (VLIST.find (n, v0) compFirst vals). simpl. eexists.
+    split. reflexivity. intro Contra. inversion Contra.
+    eexists. split. reflexivity. intro Contra. inversion Contra.
+    inversion Heqtrv.
+    eexists. split. reflexivity. intro Contra. inversion Contra.
+    inversion H. eexists. split. reflexivity. intro Contra. inversion Contra.
+Qed.
+
+Theorem progressInvokes : forall (st:DVMState) (p:Program) l m, consistentInvokes st p l m ->
+(exists st' : DVMState, INSTRUCTION.stepWith (invokes l m) st p = Some st' /\ st' <> stuck).
+Proof.
+  intros. inversion H;
+  unfold INSTRUCTION.stepWith. unfold INSTRUCTION.evalInst; unfold INSTRUCTION.evalInvokes.
+  rewrite H0. assert (filter (map l (fun x : rhs => EVAL.evalRhs x (dst frms h sh inb outb))) isNone = []).
+  eapply forAllListFilter; try apply H1. intros. eapply progressRhs. apply H6.
+  rewrite H6. remember (numberList 101
+                (map (fastRev l)
+                   (fun x : rhs =>
+                    match EVAL.evalRhs x (dst frms h sh inb outb) with
+                    | Some v1 => v1
+                    | None => ref null
+                    end))) as tlist.
+  remember (fastRev
+          (map tlist
+             (fun x : nat * Val =>
+              let (nx, vx) := x in updateFrame (upVals nx vx)))) as revMacro.
+  assert (forAllList revMacro isUpdateFrameVal). rewrite HeqrevMacro. rewrite <- rev_pres.
+  assert (forall lst',forAllList
+  (map lst'
+     (fun x : nat * Val => let (nx, vx) := x in updateFrame (upVals nx vx)))
+  isUpdateFrameVal).
+  induction lst'; simpl; econstructor. destruct a; simpl; econstructor. assumption.
+  apply H7. simpl. eapply mkChangesProgressOnUpdateFrameValPairs in H7. inversion H7.
+  eexists. split. apply H8. intro Contra; inversion Contra.
+  exists halt. split. apply mkChangesHaltsOnHalt. intro Contra; inversion Contra.
+Qed.
+
+Theorem progressInvokei : forall (st:DVMState) (p:Program) r l m, consistentInvokei st p l m r ->
+(exists st' : DVMState, INSTRUCTION.stepWith (invokei r l m) st p = Some st' /\ st' <> stuck).
+Proof.
+  intros. inversion H;
+  unfold INSTRUCTION.stepWith. unfold INSTRUCTION.evalInst; unfold INSTRUCTION.evalInvokei.
+  rewrite H0. assert (filter (map l (fun x : rhs => EVAL.evalRhs x (dst frms h sh inb outb))) isNone = []).
+  eapply forAllListFilter; try apply H1. intros. eapply progressRhs. apply H8.
+  rewrite H8. remember (numberList 101
+                (map (fastRev l)
+                   (fun x : rhs =>
+                    match EVAL.evalRhs x (dst frms h sh inb outb) with
+                    | Some v1 => v1
+                    | None => ref null
+                    end))) as tlist.
+  remember (fastRev
+          (map tlist
+             (fun x : nat * Val =>
+              let (nx, vx) := x in updateFrame (upVals nx vx)))) as revMacro.
+  assert (forAllList revMacro isUpdateFrameVal). rewrite HeqrevMacro. rewrite <- rev_pres.
+  assert (forall lst',forAllList
+  (map lst'
+     (fun x : nat * Val => let (nx, vx) := x in updateFrame (upVals nx vx)))
+  isUpdateFrameVal).
+  induction lst'; intros; simpl; econstructor. destruct a; simpl; econstructor. assumption.
+  apply H9. simpl.
+  apply progressReg in H2. destruct (EVAL.evalReg r (dst frms h sh inb outb)).
+  assert (forAllList ((updateFrame (upVals 0 v))::revMacro) isUpdateFrameVal).
+  constructor; try assumption. constructor.
+  eapply mkChangesProgressOnUpdateFrameValPairs in H10.
+  inversion H10. remember (updateFrame (upVals 0 v) :: revMacro) as tup. simpl. rewrite H11.
+  eexists. split.
+  reflexivity. intro Contra; inversion Contra.
+  inversion H2.
+  exists halt. split. apply mkChangesHaltsOnHalt. intro Contra; inversion Contra.
+Qed.
+
+Theorem progressGoto : forall (st:DVMState) (p:Program) p0, consistentGoto st p p0 ->
+  (exists st' : DVMState, INSTRUCTION.stepWith (goto p0) st p = Some st' /\ st' <> stuck).
+Proof.
+  intros; inversion H; unfold INSTRUCTION.stepWith. unfold INSTRUCTION.evalInst. unfold INSTRUCTION.evalGoto.
+  simpl. eexists. split. reflexivity. intro Contra. inversion Contra.
+  eexists halt. split. apply mkChangesHaltsOnHalt. intro Contra; inversion Contra.
+Qed.
+
+Theorem progressBranch : forall (st:DVMState) (p:Program) b p0 r r0, consistentBranch st p r r0 b p0 -> 
+  (exists st' : DVMState, INSTRUCTION.stepWith (branch r b r0 p0) st p = Some st' /\ st' <> stuck).
+Proof.
+  intros; inversion H; unfold INSTRUCTION.stepWith. unfold INSTRUCTION.evalInst. unfold INSTRUCTION.evalBranch.
+  apply EVAL.evalRhsRelEq in H0. rewrite H0.
+  apply EVAL.evalRhsRelEq in H1. rewrite H1.
+  destruct b.
+    destruct (PType.comp p2 p3 + PType.comp p3 p2)%nat.
+      simpl. eexists. split. reflexivity. intro Contra. inversion Contra.
+      inversion H2. simpl. rewrite H16. rewrite H17. simpl. eexists. split. reflexivity. intro Contra. inversion Contra.
+    destruct (PType.comp p3 p2).
+      inversion H2. simpl. rewrite H16. rewrite H17. simpl. eexists. split. reflexivity. intro Contra. inversion Contra.
+      simpl. eexists. split. reflexivity. intro Contra. inversion Contra.
+    destruct (PType.comp p2 p3).
+      inversion H2. simpl. rewrite H16. rewrite H17. simpl. eexists. split. reflexivity. intro Contra. inversion Contra.
+      simpl. eexists. split. reflexivity. intro Contra. inversion Contra.
+  exists halt. split. apply mkChangesHaltsOnHalt. intro Contra; inversion Contra.
+Qed.
+
+Theorem progressMove : forall (st:DVMState) (p:Program) r r0, consistentMove st p r r0 -> 
+  (exists st' : DVMState, INSTRUCTION.stepWith (move r r0) st p = Some st' /\ st' <> stuck).
+Proof.
+  intros; inversion H; unfold INSTRUCTION.stepWith.
+  unfold INSTRUCTION.evalInst. unfold INSTRUCTION.evalMove.
+  apply progressRhs in H0. destruct (EVAL.evalRhs r0 (dst frms h sh inb outb)).
+  inversion H1. simpl. rewrite H12. rewrite H13. simpl.
+  eexists. split. reflexivity.
+  intro Contra; inversion Contra. inversion H0.
+  exists halt. split. apply mkChangesHaltsOnHalt. intro Contra; inversion Contra.
+Qed.
+
+Theorem progressUpdate : forall (st:DVMState) (p:Program) r r0, consistentUpdate st p r r0 -> 
+  (exists st' : DVMState, INSTRUCTION.stepWith (update r r0) st p = Some st' /\ st' <> stuck).
+Proof.
+  intros; inversion H; unfold INSTRUCTION.stepWith;
+  unfold INSTRUCTION.evalInst; unfold INSTRUCTION.evalUpdate.
+  apply progressRhs in H0.
+    destruct (EVAL.evalRhs r0 (dst frms h sh inb outb)).
+      apply EVAL.evalRegRelEq in H1. rewrite H1. apply EVAL.evalRegRelEq in H2. rewrite H2.
+      apply EVAL.HP.getRelEq in H3.
+      rewrite evalHpInstHeapEq in H3. rewrite H3. apply PType.toNatRelEq in H4. rewrite H4.
+        unfold lt in H5. apply Sn_Sm_le_n_m in H5. apply isleNumProp in H5. rewrite H5.
+      inversion H6. simpl. rewrite H17. rewrite H18. simpl.
+      eexists. split. reflexivity. intro Contra; inversion Contra.
+      inversion H0.
+  apply progressRhs in H0.
+    destruct (EVAL.evalRhs r0 (dst frms h sh inb outb)).
+      apply EVAL.evalRegRelEq in H1. rewrite H1.
+      apply EVAL.HP.getRelEq in H2. rewrite evalHpInstHeapEq in H2. rewrite H2.
+      apply INSTRUCTION.FLIST.findRelEq in H3. rewrite H3. simpl.
+      inversion H4. rewrite H15. rewrite H16. simpl. eexists; split. reflexivity. intro Contra; inversion Contra.
+      inversion H0.
+  apply progressRhs in H0.
+    destruct (EVAL.evalRhs r0 (dst frms h sh inb outb)).
+      apply INSTRUCTION.FLIST.findRelEq in H1. rewrite H1. simpl.
+      inversion H2. rewrite H13. rewrite H14. simpl. eexists; split. reflexivity. intro Contra; inversion Contra.
+      inversion H0.
+  exists halt. split. apply mkChangesHaltsOnHalt. intro Contra; inversion Contra.
+Qed.
+
+Theorem progressUnary : forall (st:DVMState) (p:Program) r r0 u, consistentUnary st p r r0 u -> 
+  (exists st' : DVMState, INSTRUCTION.stepWith (unary r u r0) st p = Some st' /\ st' <> stuck).
+Proof.
+  intros; inversion H. unfold INSTRUCTION.stepWith. unfold INSTRUCTION.evalInst.
+  unfold INSTRUCTION.evalUnary. apply progressRhs in H0.
+  destruct (EVAL.evalRhs r0 (dst frms h sh inb outb)).
+  destruct v; try destruct (isle_num 1 (PType.toNat p1));
+  try destruct r2;
+    repeat (eapply progressMove;
+      constructor; try assumption; try constructor).
+  inversion H0.
+  exists halt. split. apply mkChangesHaltsOnHalt. intro Contra; inversion Contra.
+Qed.
+
+Theorem progressBinary : forall (st:DVMState) (p:Program) r r0 r1 b, consistentBinaryArith st p r r0 r1 b -> 
+  (exists st' : DVMState, INSTRUCTION.stepWith (binaryArith r r0 b r1) st p = Some st' /\ st' <> stuck).
+Proof.
+  intros; inversion H; unfold INSTRUCTION.stepWith.
+  unfold INSTRUCTION.evalInst. unfold INSTRUCTION.evalBinaryArith.
+  apply EVAL.evalRhsRelEq in H0. rewrite H0.
+  apply EVAL.evalRhsRelEq in H1. rewrite H1.
+  destruct b; repeat (eapply progressMove; constructor; try assumption; constructor).
+  exists halt. split. apply mkChangesHaltsOnHalt. intro Contra; inversion Contra.
+Qed.
+
+Theorem progressNew : forall (st:DVMState) (p:Program) r c, consistentNew st p r c -> 
+  (exists st' : DVMState, INSTRUCTION.stepWith (new r c) st p = Some st' /\ st' <> stuck).
+Proof.
+  intros; inversion H; unfold INSTRUCTION.stepWith.
+  unfold INSTRUCTION.evalInst. unfold INSTRUCTION.evalNew.
+  rewrite H0. simpl. inversion H1. rewrite H12. rewrite H13.
+  simpl. eexists. split. reflexivity. intro Contra; inversion Contra.
+  exists halt. split. apply mkChangesHaltsOnHalt. intro Contra; inversion Contra.
+Qed.
+
+Theorem progressNewArray : forall (st:DVMState) (p:Program) r t r0, consistentNewArray st p r t r0 -> 
+  (exists st' : DVMState, INSTRUCTION.stepWith (newarr r t r0) st p = Some st' /\ st' <> stuck).
+Proof.
+  intros; inversion H; unfold INSTRUCTION.stepWith.
+  unfold INSTRUCTION.evalInst. unfold INSTRUCTION.evalNewArray.
+  apply EVAL.evalRhsRelEq in H0. rewrite H0.
+  rewrite <- PType.toNatRelEq in H1. rewrite H1.
+  rewrite H2. inversion H3. simpl. rewrite H15. rewrite H16.
+  simpl. eexists. split. reflexivity. intro Contra; inversion Contra.
+  exists halt. split. apply mkChangesHaltsOnHalt. intro Contra; inversion Contra.
+Qed.
+
+Theorem progressCast : forall (st:DVMState) (p:Program) r t r0, consistentCast st p r t r0 -> 
+  (exists st' : DVMState, INSTRUCTION.stepWith (cast r t r0) st p = Some st' /\ st' <> stuck).
+Proof.
+  intros; inversion H; unfold INSTRUCTION.stepWith.
+  unfold INSTRUCTION.evalInst. unfold INSTRUCTION.evalCast.
+  apply EVAL.evalRhsRelEq in H0. rewrite H0. rewrite H1.
+  unfold TYPE.cast in H1.
+  destruct (TYPE.HEAP.get loc1 h); try inversion H1.
+  destruct t0; try inversion H1. destruct o; try inversion H1.
+  destruct t; try inversion H1. destruct r2; try inversion H1.
+  destruct (TYPE.isSub p c1 c0); try inversion H1. simpl.
+  subst. inversion H2. rewrite H14. rewrite H15. simpl.
+  eexists. split. reflexivity. intro Contra; inversion Contra.
+  exists halt. split. apply mkChangesHaltsOnHalt. intro Contra; inversion Contra.
+Qed.
+
+Theorem progressRead : forall (st:DVMState) (p:Program) r, consistentRead st p r ->
+  (exists st' : DVMState, INSTRUCTION.stepWith (read r) st p = Some st' /\ st' <> stuck).
+Proof.
+  intros; inversion H; unfold INSTRUCTION.stepWith. unfold INSTRUCTION.evalInst. unfold INSTRUCTION.evalRead.
+  simpl. apply INSTRUCTION.NLIST.getRelEq in H0. rewrite H0.
+  inversion H1. rewrite H11. rewrite H12. simpl.
+  eexists. split. reflexivity. intro Contra; inversion Contra.
+  exists halt. split. apply mkChangesHaltsOnHalt. intro Contra; inversion Contra.
+Qed.
+
+Theorem progressWrite : forall (st:DVMState) (p:Program) r, consistentWrite st p r ->
+  (exists st' : DVMState, INSTRUCTION.stepWith (print r) st p = Some st' /\ st' <> stuck).
+Proof.
+  intros; inversion H; unfold INSTRUCTION.stepWith. unfold INSTRUCTION.evalInst. unfold INSTRUCTION.evalWrite.
+  simpl. destruct outb. apply EVAL.evalRhsRelEq in H0. rewrite H0.
+  inversion H1. rewrite H11. rewrite H12. simpl.
+  eexists. split. reflexivity. intro Contra; inversion Contra.
+  exists halt. split. apply mkChangesHaltsOnHalt. intro Contra; inversion Contra.
+Qed.
+
 Theorem progress : forall (st:DVMState) (p:Program) (i:Instruction), consistentInst i st p -> 
   (exists st',INSTRUCTION.stepWith i st p = Some st' /\ ~(st' = stuck)).
 Proof.
-  destruct st.
-    intros p i.
+    intros st p.
     generalize dependent p.
     destruct i; intros; inversion H.
     (** nop *)
-      inversion H0; simpl; eapply ex_intro. split. unfold INSTRUCTION.stepWith.
-        unfold INSTRUCTION.evalInst. simpl. rewrite H9. rewrite H10. reflexivity.
-        intro. inversion H11.
+      apply progressNop. assumption.
     (** ret *)
-      inversion H0; simpl. unfold INSTRUCTION.stepWith.
-        unfold INSTRUCTION.evalInst. unfold INSTRUCTION.evalRet. rewrite H9. rewrite H10.
-        destruct (EVAL.evalReg 201 (dst (f :: frm vals ml pc :: frms0) h sh inb outb)); simpl.
-          destruct (ChangeState.VLIST.find (201, v) compFirst vals). simpl.
-          exists (dst (frm (ChangeState.VLIST.set n (201, v) vals) ml pc' :: frms0) h sh inb outb).
-          split. reflexivity. intro. inversion H11.
-          exists (dst (ChangeState.changeFrame (frm (ChangeState.VLIST.prep (201, v) vals) ml pc) (upPC pc') :: frms0) h sh inb outb).
-          split. reflexivity. intro. inversion H11.
-          exists (dst (frm vals ml pc' :: frms0) h sh inb outb).
-          split. reflexivity. intro. inversion H11.
+      apply progressRet. assumption.
     (** retTo *)
-      inversion H1; simpl. unfold INSTRUCTION.stepWith.
-        unfold INSTRUCTION.evalInst. unfold INSTRUCTION.evalRetTo. rewrite H10. rewrite H11.
-        destruct (EVAL.evalReg 201 (dst (f :: frm vals ml pc :: frms0) h sh inb outb)); simpl.
-          destruct (ChangeState.VLIST.find (201, v) compFirst vals). simpl.
-          exists (dst (ChangeState.changeFrame
-                      match ChangeState.VLIST.find (r, v) compFirst vals with
-                      | Some n' => frm (ChangeState.VLIST.set n' (r, v) vals) ml pc
-                      | None => frm (ChangeState.VLIST.prep (r, v) vals) ml pc
-                      end (upPC pc') :: frms0) h sh inb outb).
-          split. reflexivity. intro. inversion H12.
-          exists (dst (ChangeState.changeFrame
-                      match ChangeState.VLIST.find (r, v) compFirst vals with
-                      | Some n' => frm (ChangeState.VLIST.set n' (r, v) vals) ml pc
-                      | None => frm (ChangeState.VLIST.prep (r, v) vals) ml pc
-                      end (upPC pc') :: frms0) h sh inb outb).
-          split. reflexivity. intro. inversion H12.
-          exists (dst (frm vals ml pc' :: frms0) h sh inb outb).
-          split. reflexivity. intro. inversion H12.
+      apply progressRetTo. assumption.
     (** invokes *)
-      inversion H4. unfold INSTRUCTION.stepWith.
-        unfold INSTRUCTION.evalInst. unfold INSTRUCTION.evalInvokes.
-        assert ((filter (map l (fun x : rhs => EVAL.evalRhs x (dst frms h sh inb outb))) isNone) = []).
-        eapply forAllListFilter.
-        assert (forall x : rhs, (fun y:rhs => consistentEvalRhs y (dst frms h sh inb outb)) x -> isNone (EVAL.evalRhs x (dst frms h sh inb outb)) = false).
-          intros. apply progressRhs; try eassumption. eassumption. assumption.
-        rewrite H15. rewrite H13. simpl.
-        (** Resolve Here *)
-              destruct (fastRev
-       (List.map
-          (fun x : nat * Val =>
-           let (nx, vx) := x in updateFrame (upVals nx vx))
-          (numberList 101
-             (List.map
-                (fun x : rhs =>
-                 match EVAL.evalRhs x (dst frms h sh inb outb) with
-                 | Some v1 => v1
-                 | None => ref null
-                 end) (fastRev l))))). eexists. split. reflexivity.
-          intro Contra. inversion Contra.
-          simpl. unfold fastRev. simpl.
+      apply progressInvokes. assumption.
+    (** invokei *)
+      apply progressInvokei. assumption.
+    (** goto *)
+      apply progressGoto. assumption.
+    (** branch *)
+      apply progressBranch. assumption.
+    (** move *)
+      apply progressMove. assumption.
+    (** update *)
+      apply progressUpdate. assumption.
+    (** unary *)
+      apply progressUnary. replace u with uop. apply H4. destruct u. destruct uop. reflexivity.
+    (** binary *)
+      apply progressBinary. assumption.
+    (** new *)
+      apply progressNew. assumption.
+    (** newarr *)
+      apply progressNewArray. assumption.
+    (** cast *)
+      apply progressCast. assumption.
+    (** Read *)
+      apply progressRead. assumption.
+    (** W *)
+      apply progressWrite. assumption.
+Qed.
