IDvmState.v
@@ -1,6 +1,7 @@
 Require Export Defs.
 Require Export DList.
 Require Export Bvector.
+Require Export GenericState.
 
 Open Scope type_scope.
 
@@ -10,7 +11,9 @@ Parameter n:nat.
 
 Definition securityVectorType : Type := Bvector n.
 
-Inductive Frame : Type :=  frm (vals:list (nat*securityVectorType)) (ml:MethodLocation) (PC:ProgramCounter).
+Definition plusSecurityVectors := BVor n.
+
+Definition nullSecurityVector := 
 
 Inductive ObjectVectorType : Type :=
   | topObjVect : securityVectorType -> ObjectVectorType
@@ -20,37 +23,11 @@ Inductive ObjectVectorType : Type :=
 Inductive ArrayVectorType : Type :=
   | arr : nat -> list securityVectorType -> ArrayVectorType.
 
-Inductive arrOrObj : Type :=
-  | ar : ArrayVectorType -> arrOrObj
-  | dob : ObjectVectorType -> arrOrObj.
+Inductive arrOrObj' : Type :=
+  | ar : ArrayVectorType -> arrOrObj'
+  | dob : ObjectVectorType -> arrOrObj'.
 
-Definition Heap : Type := list arrOrObj.
+Declare Module IDvmStateModule : GenericStateType with Definition Val' := securityVectorType with Definition arrOrObj' := arrOrObj.  
+Export IDvmStateModule.
 
-Definition SHeap : Type := list (FieldLocation * securityVectorType).
-
-Definition Buffer : Type := Cursor*(list nat).
-
-Inductive IDVMState : Type := 
-  | dst (frms:list Frame) (h:Heap) (sh:SHeap) (inb:Buffer) (outb:Buffer)
-  | stuck
-  | halt.
-
-Inductive frameDiff : Type :=
-  | upVals : nat -> securityVectorType -> frameDiff
-  | upPC : ProgramCounter -> frameDiff.
-
-Inductive deltaState : Type :=
-  | createFrame : Frame -> deltaState
-  | updateFrame : frameDiff -> deltaState
-  | deleteFrame : deltaState
-  | addHeap : arrOrObj -> deltaState
-  | upHeap : list (nat*arrOrObj) -> deltaState
-  | upSHeap : SHeap -> deltaState
-  | addOutb : nat -> deltaState
-  | upInb : list (nat*nat) -> deltaState
-  | upOutb : list (nat*nat) -> deltaState
-  | upInc : Cursor -> deltaState
-  | upOutc : Cursor -> deltaState
-  | mkStuck : deltaState
-  | mkHalt : deltaState.
-
+End IDvmStateType.
