IEval.v
@@ -1,0 +1,332 @@
+Require Export IDvmState.
+Require Export Program.
+
+(**
+
+* Overview
+
+This Module implements functionality to evaluate simple expressions that occur in CoqDVM instruction provided current state
+
+* EVALTYPE signature
+
+Here we have just three function prototypes
+- evalReg : evaluates value of a register
+- evalLhs : evaluates value of lhs expression
+- evalRhs : evaluates value of rhs expression
+
+*)
+
+
+Module Type IEVALTYPE.
+  Parameter n : nat.
+  Parameter DVMState : Type.
+  Parameter Val : Type.
+  Parameter arrOrObj : Type.
+  Parameter evalReg : nat -> DVMState -> @Option Val.
+  Parameter evalLhs : lhs -> DVMState -> @Option Val.
+  Parameter evalRhs : rhs -> DVMState -> @Option Val.
+End IEVALTYPE.
+
+(**
+
+* EVAL module
+
+*)
+
+Module IEVAL <: IEVALTYPE.
+
+Parameter n : nat.
+
+Declare Module IDvmStateMod : IDvmStateType with Definition n := n.
+Export IDvmStateMod.
+
+Definition DVMState : Type := State.
+Definition Val := Val'.
+Definition arrOrObj := arrOrObj'.
+
+(**
+
+List Based Declarions to be used later.
+
+*)
+  Declare Module RLIST : ListType with Definition t1 := nat*Val.
+  Declare Module HP : ListType with Definition t1 := arrOrObj.
+  Declare Module VLIST : ListType with Definition t1 := Val.
+  Declare Module LVLIST : ListType with Definition t1 := (FieldLocation*Val).
+  Declare Module SVLIST : ListType with Definition t1 := (FieldLocation*Val).
+
+(**
+
+** evalReg : Evaluates Register
+
+*)
+
+  Fixpoint evalReg (n:nat) (st:DVMState) : @Option Val :=
+    match st with
+    | dst nil h sh inb outb => None
+    | dst (cons (frm lst m pc) frem) h sh inb outb => match (RLIST.find (n,(ref null)) compFirst lst) with
+      | (Some n') => match (RLIST.get n' lst) with
+        | (Some (z,x)) => Some x
+        | None => None
+        end
+      | None => None
+      end
+    | stuck => None
+    | halt => None
+    end.
+
+  Inductive evalRegRel : nat -> DVMState -> @Option Val -> Prop :=
+    | nilEvalRegRel : forall (n:nat) (h:Heap) (sh:SHeap) (inb outb:Buffer), evalRegRel n (dst nil h sh inb outb) None
+    | someSomeEvalRegRel : forall (n n' n'':nat) (x:Val) (frem:list Frame) (lst:list (nat*Val)) (m:MethodLocation) (pc:ProgramCounter) (h:Heap) (sh:SHeap) (inb outb:Buffer),
+                      RLIST.findRel (n,(ref null)) compFirst lst (Some n') ->
+                      RLIST.getRel n' lst (Some (n'',x)) ->
+                      evalRegRel n (dst (cons (frm lst m pc) frem) h sh inb outb) (Some x)
+    | someNoneEvalRegRel : forall (n n':nat) (frem:list Frame) (lst:list (nat*Val)) (m:MethodLocation) (pc:ProgramCounter) (h:Heap) (sh:SHeap) (inb outb:Buffer),
+                      RLIST.findRel (n,(ref null)) compFirst lst (Some n') ->
+                      RLIST.getRel n' lst None ->
+                      evalRegRel n (dst (cons (frm lst m pc) frem) h sh inb outb) None
+    | noneEvalRegRel : forall (n:nat) (frem:list Frame) (lst:list (nat*Val)) (m:MethodLocation) (pc:ProgramCounter) (h:Heap) (sh:SHeap) (inb outb:Buffer),
+                      RLIST.findRel (n,(ref null)) compFirst lst None ->
+                      evalRegRel n (dst (cons (frm lst m pc) frem) h sh inb outb) None
+    | stuckEvalRegRel : forall (n:nat), evalRegRel n stuck None
+    | haltEvalRegRel : forall (n:nat), evalRegRel n halt None.
+
+  Theorem evalRegRelEq : forall (n:nat) (st:DVMState) (v1:@Option Val), evalReg n st = v1 <-> evalRegRel n st v1.
+  Proof.
+    split; intro.
+    destruct st; simpl in H; subst; simpl; try (destruct n; simpl; econstructor). 
+    destruct frms; simpl.
+      destruct n; simpl; econstructor.
+      destruct n; simpl; destruct f; simpl.
+      remember (RLIST.find (0, ref null) compFirst vals) as fres; destruct fres; symmetry in Heqfres;
+      apply RLIST.findRelEq in Heqfres; try constructor; auto.
+      remember (RLIST.get n vals) as gres; destruct gres; symmetry in Heqgres; apply RLIST.getRelEq in Heqgres.
+      destruct t. econstructor. eapply Heqfres. eapply Heqgres.
+      eapply someNoneEvalRegRel. eapply Heqfres. apply Heqgres.
+      remember (RLIST.find ((S n), ref null) compFirst vals) as fres; destruct fres; symmetry in Heqfres;
+      apply RLIST.findRelEq in Heqfres; try constructor; auto.
+      remember (RLIST.get n0 vals) as gres; destruct gres; symmetry in Heqgres; apply RLIST.getRelEq in Heqgres.
+      destruct t. econstructor. eapply Heqfres. eapply Heqgres.
+      eapply someNoneEvalRegRel. eapply Heqfres. apply Heqgres.
+    inversion H; subst; destruct n; simpl; try reflexivity;
+      try (apply RLIST.findRelEq in H0; rewrite H0; try reflexivity; apply RLIST.getRelEq in H1; rewrite H1; reflexivity).
+  Qed.
+
+(**
+
+** evalLhs : Evaluates lhs expressions
+
+*)
+
+  Definition evalLhs (exp:lhs) (st:DVMState) : @Option Val :=
+    match exp,st with
+    | (reg n),x => evalReg n st
+    | (acc n n2),dst frms h sh inb outb => match (evalReg n st) with
+      | Some (ref (lRef lc)) => match (HP.get lc h),(evalReg n2 st) with
+        | Some (ar (arr n' lst)),(Some (prim p1)) => (VLIST.get (PType.toNat p1) lst)
+        | x,y => None
+        end
+      | x => None
+      end
+    | (ifield n1 n2),(dst frms h sh inb outb) => match (evalReg n1 st) with
+      | Some (ref (lRef lc)) => match (HP.get lc h) with
+        | Some (dob (obj n' n'' lst)) => match (LVLIST.find (n2,(ref null)) compFirst lst) with
+          | Some n3 => match (LVLIST.get n3 lst) with
+            | Some (n',vl') => Some vl'
+            | None => None
+            end
+          | x => None
+          end
+        | x => None
+        end
+      | x => None
+      end
+    | (sfield n),(dst frms h sh inb outb) => match (SVLIST.find (n,(ref null)) compFirst sh) with
+      | Some n2 => match (SVLIST.get n2 sh) with
+        | Some (n3,v') => Some v'
+        | None => None
+        end
+      | None => None
+      end
+    | x , y => None
+    end.
+
+  Inductive evalLhsRel : lhs -> DVMState -> @Option Val -> Prop :=
+    | regEvalLhsRel : forall (n:nat) (st:DVMState) (v:@Option Val), evalRegRel n st v -> evalLhsRel (reg n) st v
+    | noneFirstAccEvalLhsRel : forall (n n2:nat) (st:DVMState), evalRegRel n st None -> evalLhsRel (acc n n2) st None
+    | somePrimFirstAccEvalLhsRel : forall (n n2:nat) (p:Prim) (st:DVMState), evalRegRel n st (Some (prim p)) -> evalLhsRel (acc n n2) st None
+    | someNullFirstAccEvalLhsRel : forall (n n2:nat) (st:DVMState), evalRegRel n st (Some (ref null)) -> evalLhsRel (acc n n2) st None
+    | noneSecondAccEvalLhsRel : forall (n n2:nat) (st:DVMState), evalRegRel n2 st None -> evalLhsRel (acc n n2) st None
+    | someRefSecondAccEvalLhsRel : forall (n n2:nat) (r:Ref) (st:DVMState), evalRegRel n2 st (Some (ref r)) -> evalLhsRel (acc n n2) st None
+    | someNoneAccEvalLhsRel : forall (n n2:nat) (lc:Location) (frms:list Frame) (h:Heap) (sh:SHeap) (inb outb:Buffer),
+                              evalRegRel n (dst frms h sh inb outb) (Some (ref (lRef lc))) ->
+                              HP.getRel lc h None ->
+                              evalLhsRel (acc n n2) (dst frms h sh inb outb) None
+    | someSomeDobAccEvalLhsRel : forall (n n2:nat) (lc:Location) (object:Object) (frms:list Frame) (h:Heap) (sh:SHeap) (inb outb:Buffer),
+                              evalRegRel n (dst frms h sh inb outb) (Some (ref (lRef lc))) ->
+                              HP.getRel lc h (Some (dob object)) ->
+                              evalLhsRel (acc n n2) (dst frms h sh inb outb) None
+    | someSomeArAccEvalLhsRel : forall (n n1 n2 n':nat) (lc:Location) (p1:Prim) (frms:list Frame) (h:Heap) (sh:SHeap) (inb outb:Buffer) (v:@Option Val) (lst:list Val),
+                              evalRegRel n (dst frms h sh inb outb) (Some (ref (lRef lc))) ->
+                              HP.getRel lc h (Some (ar (arr n' lst))) ->
+                              evalRegRel n2 (dst frms h sh inb outb) (Some (prim p1)) ->
+                              PType.toNatRel p1 n1 ->
+                              VLIST.getRel n1 lst v ->
+                              evalLhsRel (acc n n2) (dst frms h sh inb outb) v
+    | noneFirstIfieldEvalLhsRel : forall (n1 n2:nat) (st:DVMState), evalRegRel n1 st None -> evalLhsRel (ifield n1 n2) st None
+    | somePrimFirstIfieldEvalLhsRel : forall (n1 n2:nat) (st:DVMState) (p1:Prim), evalRegRel n1 st (Some (prim p1)) -> evalLhsRel (ifield n1 n2) st None
+    | someNullFirstIfieldEvalLhsRel : forall (n1 n2:nat) (st:DVMState), evalRegRel n1 st (Some (ref null)) -> evalLhsRel (ifield n1 n2) st None
+    | someNoneIfieldEvalLhsRel : forall (n1 n2:nat) (lc:Location) (frms:list Frame) (h:Heap) (sh:SHeap) (inb outb:Buffer),
+                              evalRegRel n1 (dst frms h sh inb outb) (Some (ref (lRef lc))) ->
+                              HP.getRel lc h None ->
+                              evalLhsRel (ifield n1 n2) (dst frms h sh inb outb) None
+    | someArIfieldEvalLhsRel : forall (n1 n2:nat) (array:Array) (lc:Location) (frms:list Frame) (h:Heap) (sh:SHeap) (inb outb:Buffer),
+                              evalRegRel n1 (dst frms h sh inb outb) (Some (ref (lRef lc))) ->
+                              HP.getRel lc h (Some (ar array)) ->
+                              evalLhsRel (ifield n1 n2) (dst frms h sh inb outb) None
+    | someTopIfieldEvalLhsRel : forall (n1 n2:nat) (lc:Location) (frms:list Frame) (h:Heap) (sh:SHeap) (inb outb:Buffer),
+                              evalRegRel n1 (dst frms h sh inb outb) (Some (ref (lRef lc))) ->
+                              HP.getRel lc h (Some (dob topObj)) ->
+                              evalLhsRel (ifield n1 n2) (dst frms h sh inb outb) None
+    | someDobjIfieldEvalLhsRel : forall (n1 n2:nat) (lc:Location) (frms:list Frame) (h:Heap) (sh:SHeap) (inb outb:Buffer),
+                              evalRegRel n1 (dst frms h sh inb outb) (Some (ref (lRef lc))) ->
+                              HP.getRel lc h (Some (dob dobj)) ->
+                              evalLhsRel (ifield n1 n2) (dst frms h sh inb outb) None
+    | someObjNoneIfieldEvalLhsRel : forall (n1 n3 n4:nat) (n2:FieldLocation) (lc:Location) (frms:list Frame) (h:Heap) (sh:SHeap) (inb outb:Buffer) (lst:list (FieldLocation*Val)),
+                              evalRegRel n1 (dst frms h sh inb outb) (Some (ref (lRef lc))) ->
+                              HP.getRel lc h (Some (dob (obj n3 n4 lst))) ->
+                              LVLIST.findRel (n2,(ref null)) compFirst lst None ->
+                              evalLhsRel (ifield n1 n2) (dst frms h sh inb outb) None
+    | someObjSomeNoneIfieldEvalLhsRel : forall (n1 n3 n4 n5:nat) (lc:Location) (n2:FieldLocation) (frms:list Frame) (h:Heap) (sh:SHeap) (inb outb:Buffer) (lst:list (FieldLocation*Val)),
+                              evalRegRel n1 (dst frms h sh inb outb) (Some (ref (lRef lc))) ->
+                              HP.getRel lc h (Some (dob (obj n3 n4 lst))) ->
+                              LVLIST.findRel (n2,(ref null)) compFirst lst (Some n5) ->
+                              LVLIST.getRel n5 lst None ->
+                              evalLhsRel (ifield n1 n2) (dst frms h sh inb outb) None
+    | someObjSomeSomeIfieldEvalLhsRel : forall (n1 n3 n4 n5 n6:nat) (lc:Location) (n2:FieldLocation) (frms:list Frame) (h:Heap) (sh:SHeap) (inb outb:Buffer) (lst:list (FieldLocation*Val)) (v1:Val),
+                              evalRegRel n1 (dst frms h sh inb outb) (Some (ref (lRef lc))) ->
+                              HP.getRel lc h (Some (dob (obj n3 n4 lst))) ->
+                              LVLIST.findRel (n2,(ref null)) compFirst lst (Some n5) ->
+                              LVLIST.getRel n5 lst (Some (n6,v1)) ->
+                              evalLhsRel (ifield n1 n2) (dst frms h sh inb outb) (Some v1)
+    | noneSfieldEvalLhsRel : forall (n:FieldLocation) (frms:list Frame) (h:Heap) (sh:SHeap) (inb outb:Buffer),
+                              SVLIST.findRel (n,(ref null)) compFirst sh None ->
+                              evalLhsRel (sfield n) (dst frms h sh inb outb) None
+    | someNoneSfieldEvalLhsRel : forall (n:FieldLocation) (n2:nat) (frms:list Frame) (h:Heap) (sh:SHeap) (inb outb:Buffer),
+                              SVLIST.findRel (n,(ref null)) compFirst sh (Some n2) ->
+                              SVLIST.getRel n2 sh None ->
+                              evalLhsRel (sfield n) (dst frms h sh inb outb) None
+    | someSomeSfieldEvalLhsRel : forall (n:FieldLocation) (n2 n3:nat) (frms:list Frame) (h:Heap) (sh:SHeap) (inb outb:Buffer) (v1:Val),
+                              SVLIST.findRel (n,(ref null)) compFirst sh (Some n2) ->
+                              SVLIST.getRel n2 sh (Some (n3,v1)) ->
+                              evalLhsRel (sfield n) (dst frms h sh inb outb) (Some v1)
+    | stuckEvalLhsRel : forall (l1:lhs), evalLhsRel l1 stuck None
+    | haltEvalLhsRel : forall (l1:lhs), evalLhsRel l1 halt None.
+
+  Theorem evalLhsRelEq : forall (l1:lhs) (st:DVMState) (v1:@Option Val), evalLhs l1 st = v1 <-> evalLhsRel l1 st v1.
+  Proof.
+    split; intro.
+    destruct st; simpl in H; subst; destruct l1; simpl; try constructor; (try (destruct r; constructor)).
+    remember (evalReg r (dst frms h sh inb outb)) as eregr. destruct eregr; symmetry in Heqeregr; apply evalRegRelEq in Heqeregr; assumption.
+    remember (evalReg r (dst frms h sh inb outb)) as eregr. destruct eregr; symmetry in Heqeregr; try (apply evalRegRelEq in Heqeregr; apply noneFirstAccEvalLhsRel; assumption).
+    destruct v. eapply somePrimFirstAccEvalLhsRel. eapply evalRegRelEq. eauto.
+    destruct r1; (try (apply someNullFirstAccEvalLhsRel; apply evalRegRelEq; auto)).
+    remember (HP.get l h) as getl. destruct getl; symmetry in Heqgetl; apply HP.getRelEq in Heqgetl.
+      destruct t. destruct a.
+        remember (evalReg r0 (dst frms h sh inb outb)) as eregr0. destruct eregr0; symmetry in Heqeregr0; apply evalRegRelEq in Heqeregr0.
+          destruct v. remember (VLIST.get (PType.toNat p) l0) as get2. symmetry in Heqget2. remember (PType.toNat p) as n'. symmetry in Heqn'.
+          eapply someSomeArAccEvalLhsRel. eapply evalRegRelEq. eapply Heqeregr. eapply Heqgetl. apply Heqeregr0. eapply PType.toNatRelEq. eapply Heqn'.
+          eapply VLIST.getRelEq. assumption. eapply someRefSecondAccEvalLhsRel. eapply Heqeregr0.
+          eapply noneSecondAccEvalLhsRel. assumption. 
+          remember (evalReg r0 (dst frms h sh inb outb)) as eregr0. destruct eregr0; symmetry in Heqeregr0.
+            eapply someSomeDobAccEvalLhsRel. eapply evalRegRelEq. eapply Heqeregr. eapply Heqgetl.
+          eapply noneSecondAccEvalLhsRel. eapply evalRegRelEq. assumption.
+          eapply someNoneAccEvalLhsRel. eapply evalRegRelEq. eapply Heqeregr. assumption.
+    remember (evalReg r (dst frms h sh inb outb)) as eregr. destruct eregr; symmetry in Heqeregr; apply evalRegRelEq in Heqeregr; (try (eapply noneFirstIfieldEvalLhsRel; assumption)).
+    destruct v. eapply somePrimFirstIfieldEvalLhsRel. apply Heqeregr.
+    destruct r0. remember (HP.get l h) as getl. symmetry in Heqgetl. apply HP.getRelEq in Heqgetl. destruct getl.
+    destruct t. eapply someArIfieldEvalLhsRel. apply Heqeregr. apply Heqgetl.
+    destruct o. eapply someTopIfieldEvalLhsRel. apply Heqeregr. assumption.
+    remember (LVLIST.find (f, ref null) compFirst l0) as fres. symmetry in Heqfres. apply LVLIST.findRelEq in Heqfres.
+    destruct fres. remember (LVLIST.get n l0) as getl0. symmetry in Heqgetl0. apply LVLIST.getRelEq in Heqgetl0. destruct getl0.
+    destruct t. eapply someObjSomeSomeIfieldEvalLhsRel. eapply Heqeregr. eapply Heqgetl. eapply Heqfres. eapply Heqgetl0.
+    eapply someObjSomeNoneIfieldEvalLhsRel. eapply Heqeregr. eapply Heqgetl. eapply Heqfres. eapply Heqgetl0.
+    eapply someObjNoneIfieldEvalLhsRel. eapply Heqeregr. eapply Heqgetl. eapply Heqfres.
+    eapply someDobjIfieldEvalLhsRel. eapply Heqeregr. eapply Heqgetl.
+    eapply someNoneIfieldEvalLhsRel. eapply Heqeregr. eapply Heqgetl.
+    apply someNullFirstIfieldEvalLhsRel. assumption.
+    remember (SVLIST.find (f, ref null) compFirst sh) as fres. symmetry in Heqfres. apply SVLIST.findRelEq in Heqfres.
+    destruct fres. remember (SVLIST.get n sh) as getn. symmetry in Heqgetn. apply SVLIST.getRelEq in Heqgetn.
+    destruct getn. destruct t. eapply someSomeSfieldEvalLhsRel. eapply Heqfres. eapply Heqgetn.
+    eapply someNoneSfieldEvalLhsRel. eapply Heqfres. assumption.
+    eapply noneSfieldEvalLhsRel. assumption.
+    (* If part done *)
+    inversion H; simpl.
+      apply evalRegRelEq in H0; rewrite H0; reflexivity.
+      apply evalRegRelEq in H0; rewrite H0; destruct st; reflexivity.
+      apply evalRegRelEq in H0; rewrite H0; destruct st; reflexivity.
+      apply evalRegRelEq in H0; rewrite H0; destruct st; reflexivity.
+      apply evalRegRelEq in H0; rewrite H0; destruct st; try reflexivity. destruct (evalReg n (dst frms h sh inb outb)); destruct v; auto; destruct r; auto. destruct (HP.get l h); auto. destruct t; auto. destruct a; auto.
+      apply evalRegRelEq in H0; rewrite H0; destruct st; try reflexivity. destruct (evalReg n (dst frms h sh inb outb)); destruct v; auto; destruct r0; auto. destruct (HP.get l h); auto. destruct t; auto. destruct a; auto.
+      apply evalRegRelEq in H0; rewrite H0. eapply HP.getRelEq in H1. rewrite H1. reflexivity.
+      apply evalRegRelEq in H0; rewrite H0. eapply HP.getRelEq in H1. rewrite H1. reflexivity.
+      apply evalRegRelEq in H0; rewrite H0. eapply HP.getRelEq in H1. rewrite H1. apply evalRegRelEq in H2. rewrite H2. apply PType.toNatRelEq in H3. rewrite H3. apply VLIST.getRelEq. assumption.
+      destruct st; auto; apply evalRegRelEq in H0; rewrite H0; auto.
+      destruct st; auto; apply evalRegRelEq in H0; rewrite H0; auto.
+      destruct st; auto; apply evalRegRelEq in H0; rewrite H0; auto.
+      apply evalRegRelEq in H0; rewrite H0; auto. apply HP.getRelEq in H1. rewrite H1. reflexivity.
+      apply evalRegRelEq in H0; rewrite H0; auto. apply HP.getRelEq in H1. rewrite H1. reflexivity.
+      apply evalRegRelEq in H0; rewrite H0; auto. apply HP.getRelEq in H1. rewrite H1. reflexivity.
+      apply evalRegRelEq in H0; rewrite H0; auto. apply HP.getRelEq in H1. rewrite H1. reflexivity.
+      apply evalRegRelEq in H0; rewrite H0; auto. apply HP.getRelEq in H1. rewrite H1.
+      apply LVLIST.findRelEq in H2. rewrite H2. reflexivity.
+      apply evalRegRelEq in H0; rewrite H0; auto. apply HP.getRelEq in H1. rewrite H1. apply LVLIST.findRelEq in H2. rewrite H2. apply LVLIST.getRelEq in H3. rewrite H3. reflexivity.
+      apply evalRegRelEq in H0; rewrite H0; auto. apply HP.getRelEq in H1. rewrite H1. apply LVLIST.findRelEq in H2. rewrite H2. apply LVLIST.getRelEq in H3. rewrite H3. reflexivity.
+      apply SVLIST.findRelEq in H0. rewrite H0. reflexivity.
+      apply SVLIST.findRelEq in H0. rewrite H0. apply SVLIST.getRelEq in H1. rewrite H1. reflexivity.
+      apply SVLIST.findRelEq in H0. rewrite H0. apply SVLIST.getRelEq in H1. rewrite H1. reflexivity.
+      destruct l1; simpl; auto. apply evalRegRelEq. constructor.
+      destruct l1; simpl; auto. apply evalRegRelEq. constructor.
+  Qed.
+(* ShortCuts
+      try (destruct st; simpl; reflexivity); try (apply HP.getRelEq in H1; rewrite H1; simpl; auto); try (destruct l1; simpl; reflexivity).
+      destruct st; try reflexivity. destruct (evalReg n (dst frms h sh inb outb)); destruct v; simpl; try reflexivity. destruct r; auto. destruct (HP.get l h); auto. destruct t; auto. destruct a; auto.
+      destruct st; try reflexivity. destruct (evalReg n (dst frms h sh inb outb)); destruct v; simpl; try reflexivity. destruct r0; auto. destruct (HP.get l h); auto. destruct t; auto. destruct a; auto.
+      apply evalRegRelEq in H2. rewrite H2. apply PType.toNatRelEq in H3. rewrite H3. apply VLIST.getRelEq. assumption.
+*)
+
+(* Bug Alert ! pattern matching bug *)
+
+(**
+
+** evalRhs : Evaluates rhs expressions
+
+*)
+
+  Definition evalRhs (exp:rhs) (st:DVMState) : @Option Val :=
+    match exp with
+    | (l lhs1) => (evalLhs lhs1 st)
+    | (cs cnst) => match cnst with
+      | cnat n => Some (prim (int n))
+      | ctrue => Some (prim (boolean 1))
+      | cfalse => Some (prim (boolean 0))
+      | cnull => Some (ref null)
+      end
+    end.
+
+  Inductive evalRhsRel : rhs -> DVMState -> @Option Val -> Prop :=
+    | lhsEvalRhsRel : forall (l1:lhs) (st:DVMState) (v:@Option Val), evalLhsRel l1 st v -> evalRhsRel (l l1) st v
+    | cnatEvalRhsRel : forall (n:nat) (st:DVMState), evalRhsRel (cs (cnat n)) st (Some (prim (int n)))
+    | ctrueEvalRhsRel : forall (st:DVMState), evalRhsRel (cs ctrue) st (Some (prim (boolean 1)))
+    | cfalseEvalRhsRel : forall (st:DVMState), evalRhsRel (cs cfalse) st (Some (prim (boolean 0)))
+    | cnullEvalRhsRel : forall (st:DVMState), evalRhsRel (cs cnull) st (Some (ref null)).
+
+  Theorem evalRhsRelEq : forall (r1:rhs) (st:DVMState) (v1:@Option Val), evalRhs r1 st = v1 <-> evalRhsRel r1 st v1.
+  Proof.
+    split; intro.
+    destruct r1. simpl in H. apply evalLhsRelEq in H. constructor. assumption.
+    destruct c; simpl in H; rewrite <- H; constructor.
+    inversion H; simpl; auto. apply evalLhsRelEq. assumption.
+  Qed.
+
+End IEVAL.
